LeanLambdaLib/LambdaLib/paperexamples.lean
@@ -1,0 +1,18 @@
+inductive ty : Type where
+| arrow : ty → ty → ty
+| base : ty
+
+def Γ := List ty
+
+inductive Var : Γ → ty → Type where
+| zero : ∀ {Γ ty}, Var (ty :: Γ) ty
+| succ : ∀ {Γ A B}, Var Γ A → Var (B :: Γ) A
+
+inductive Deriv : Γ → ty → Type where
+| var : ∀ {Γ ty}, Var Γ ty → Deriv Γ ty
+| lambda : ∀ {Γ A B}, Deriv (A :: Γ) B → Deriv Γ (.arrow A B)
+| app : ∀ {Γ A B}, Deriv Γ (.arrow A B) → Deriv Γ A → Deriv Γ B
+| tt : ∀ {Γ}, Deriv Γ .base
+
+def prog : Deriv [] (.arrow (.arrow .base .base) (.arrow .base .base)) :=
+  .lambda (.lambda (.app (.var (.succ .zero)) (.var .zero)))
